split the compiler
git-svn-id: https://projects.brucker.ch/hol-testgen/svn/HOL-TestGen/trunk/hol-testgen@10554 3260e6d1-4efc-4170-b0a7-36055960796d

src/OCL_compiler_parser_init.thy
@@ -44,7 +44,7 @@
 header{* Part ... *}
 
 theory  OCL_compiler_parser_init
-imports OCL_compiler_meta_Pure
+imports OCL_compiler_init
 begin
 
 definition "K x _ = x"
@@ -121,31 +121,6 @@ definition "i_of_option a b f = option_rec
 
 (* *)
 
-definition "i_of_pure_indexname a b = pure_indexname_rec
-  (ap2 a (b ''PureIndexname'') (i_of_string a b) (i_of_nat a b))"
-
-definition "i_of_pure_class a b = pure_class_rec
-  (ap1 a (b ''PureClass'') (i_of_string a b))"
-
-definition "i_of_pure_sort a b = pure_sort_rec
-  (ap1 a (b ''PureSort'') (i_of_list a b (i_of_pure_class a b)))"
-
-definition "i_of_pure_typ a b = (\<lambda>f1 f2 f3 f4 f5. pure_typ_rec_1 (co1 K f1) f2 f3 f4 (\<lambda>_ _. f5))
-  (ar2 a (b ''PureType'') (i_of_string a b))
-  (ap2 a (b ''PureTFree'') (i_of_string a b) (i_of_pure_sort a b))
-  (ap2 a (b ''PureTVar'') (i_of_pure_indexname a b) (i_of_pure_sort a b))
-  (* *)
-  (b i_Nil)
-  (ar2 a (b i_Cons) id)"
-
-definition "i_of_pure_term a b = (\<lambda>f0 f1 f2 f3 f4 f5. pure_term_rec f0 f1 f2 f3 (co2 K f4) (\<lambda>_ _. f5))
-  (ap2 a (b ''PureConst'') (i_of_string a b) (i_of_pure_typ a b))
-  (ap2 a (b ''PureFree'') (i_of_string a b) (i_of_pure_typ a b))
-  (ap2 a (b ''PureVar'') (i_of_pure_indexname a b) (i_of_pure_typ a b))
-  (ap1 a (b ''PureBound'') (i_of_nat a b))
-  (ar3 a (b ''PureAbs'') (i_of_string a b) (i_of_pure_typ a b))
-  (ar2 a (b ''PureApp'') id)"
-
 definition "i_of_internal_oid a b = internal_oid_rec
   (ap1 a (b ''Oid'') (i_of_nat a b))"
 
@@ -162,11 +137,6 @@ lemmas [code] =
   i_of.i_of_list_def
   i_of.i_of_option_def
   (* *)
-  i_of.i_of_pure_indexname_def
-  i_of.i_of_pure_class_def
-  i_of.i_of_pure_sort_def
-  i_of.i_of_pure_typ_def
-  i_of.i_of_pure_term_def
   i_of.i_of_internal_oid_def
   i_of.i_of_internal_oids_def
 
