src/OCL_compiler_parser_Pure.thy
@@ -1,0 +1,92 @@
+(*****************************************************************************
+ * Featherweight-OCL --- A Formal Semantics for UML-OCL Version OCL 2.4
+ *                       for the OMG Standard.
+ *                       http://www.brucker.ch/projects/hol-testgen/
+ *
+ * OCL_compiler_parser_Pure.thy ---
+ * This file is part of HOL-TestGen.
+ *
+ * Copyright (c) 2013-2014 Universite Paris-Sud, France
+ *               2013-2014 IRT SystemX, France
+ *
+ * All rights reserved.
+ *
+ * Redistribution and use in source and binary forms, with or without
+ * modification, are permitted provided that the following conditions are
+ * met:
+ *
+ *     * Redistributions of source code must retain the above copyright
+ *       notice, this list of conditions and the following disclaimer.
+ *
+ *     * Redistributions in binary form must reproduce the above
+ *       copyright notice, this list of conditions and the following
+ *       disclaimer in the documentation and/or other materials provided
+ *       with the distribution.
+ *
+ *     * Neither the name of the copyright holders nor the names of its
+ *       contributors may be used to endorse or promote products derived
+ *       from this software without specific prior written permission.
+ *
+ * THIS SOFTWARE IS PROVIDED BY THE COPYRIGHT HOLDERS AND CONTRIBUTORS
+ * "AS IS" AND ANY EXPRESS OR IMPLIED WARRANTIES, INCLUDING, BUT NOT
+ * LIMITED TO, THE IMPLIED WARRANTIES OF MERCHANTABILITY AND FITNESS FOR
+ * A PARTICULAR PURPOSE ARE DISCLAIMED. IN NO EVENT SHALL THE COPYRIGHT
+ * OWNER OR CONTRIBUTORS BE LIABLE FOR ANY DIRECT, INDIRECT, INCIDENTAL,
+ * SPECIAL, EXEMPLARY, OR CONSEQUENTIAL DAMAGES (INCLUDING, BUT NOT
+ * LIMITED TO, PROCUREMENT OF SUBSTITUTE GOODS OR SERVICES; LOSS OF USE,
+ * DATA, OR PROFITS; OR BUSINESS INTERRUPTION) HOWEVER CAUSED AND ON ANY
+ * THEORY OF LIABILITY, WHETHER IN CONTRACT, STRICT LIABILITY, OR TORT
+ * (INCLUDING NEGLIGENCE OR OTHERWISE) ARISING IN ANY WAY OUT OF THE USE
+ * OF THIS SOFTWARE, EVEN IF ADVISED OF THE POSSIBILITY OF SUCH DAMAGE.
+ ******************************************************************************)
+(* $Id:$ *)
+
+header{* Part ... *}
+
+theory  OCL_compiler_parser_Pure
+imports OCL_compiler_meta_Pure
+        OCL_compiler_parser_init
+begin
+
+subsection{* i of ... *} (* i_of *)
+
+subsubsection{* general *}
+
+context i_of
+begin
+
+definition "i_of_pure_indexname a b = pure_indexname_rec
+  (ap2 a (b ''PureIndexname'') (i_of_string a b) (i_of_nat a b))"
+
+definition "i_of_pure_class a b = pure_class_rec
+  (ap1 a (b ''PureClass'') (i_of_string a b))"
+
+definition "i_of_pure_sort a b = pure_sort_rec
+  (ap1 a (b ''PureSort'') (i_of_list a b (i_of_pure_class a b)))"
+
+definition "i_of_pure_typ a b = (\<lambda>f1 f2 f3 f4 f5. pure_typ_rec_1 (co1 K f1) f2 f3 f4 (\<lambda>_ _. f5))
+  (ar2 a (b ''PureType'') (i_of_string a b))
+  (ap2 a (b ''PureTFree'') (i_of_string a b) (i_of_pure_sort a b))
+  (ap2 a (b ''PureTVar'') (i_of_pure_indexname a b) (i_of_pure_sort a b))
+  (* *)
+  (b i_Nil)
+  (ar2 a (b i_Cons) id)"
+
+definition "i_of_pure_term a b = (\<lambda>f0 f1 f2 f3 f4 f5. pure_term_rec f0 f1 f2 f3 (co2 K f4) (\<lambda>_ _. f5))
+  (ap2 a (b ''PureConst'') (i_of_string a b) (i_of_pure_typ a b))
+  (ap2 a (b ''PureFree'') (i_of_string a b) (i_of_pure_typ a b))
+  (ap2 a (b ''PureVar'') (i_of_pure_indexname a b) (i_of_pure_typ a b))
+  (ap1 a (b ''PureBound'') (i_of_nat a b))
+  (ar3 a (b ''PureAbs'') (i_of_string a b) (i_of_pure_typ a b))
+  (ar2 a (b ''PureApp'') id)"
+
+end
+
+lemmas [code] =
+  i_of.i_of_pure_indexname_def
+  i_of.i_of_pure_class_def
+  i_of.i_of_pure_sort_def
+  i_of.i_of_pure_typ_def
+  i_of.i_of_pure_term_def
+
+end
